test.thy
@@ -305,8 +305,278 @@ qed
 
 lemma n_common_prefix:
   "\<forall>r r'. nCheck n d t \<and> r\<in>nLongest t \<and> r'\<in>nLongest t \<longrightarrow> take n r = take n r'"
-sorry
+proof (induction n arbitrary: t)
+  case 0
+  then show ?case by simp
+next
+  case (Suc n)
+  show ?case
+  proof (rule allI impI)+
+    fix r r'
+    assume a1 : "nCheck (Suc n) d t \<and> r \<in> nLongest t \<and> r' \<in> nLongest t"
+    then have *: "nCheck (Suc n) d t" and **: "r \<in> nLongest t" and ***: "r' \<in> nLongest t" by auto
+    obtain v xs where t_def: "t = nNode v xs" using nTree.exhaust by auto
 
+    then obtain p where p_def: "p \<in> set xs"
+      and height_cond: "\<forall>p' \<in> set xs - {p}. nHeight p - nHeight p' > d"
+      and check_p: "nCheck n d p" using * t_def by fastforce
 
+    have ****:"\<forall>t''\<in>set xs - {p}. nHeight t'' < nHeight p" using height_cond by force
 
+    then obtain p' where " p' \<in> nLongest p" and r_def: "r = v # p'"
+      by (smt (verit, best) "**" sub_branch list.set_cases p_def t_def) 
+    (*Show the tail of longest paths are in p*)
+    then have r_in_p: "tl r \<in> nLongest p" by auto
+    
+    from **** obtain p'' where "p'' \<in> nLongest p" and r'_def:  "r' = v # p''" 
+      by (smt (verit, ccfv_SIG) "***" sub_branch list.set_cases p_def t_def)  
+
+    then have r'_in_p: "tl r' \<in> nLongest p" by auto
+    then have take_tl : "take n (tl r) = take n (tl r')" using Suc check_p r'_in_p r_in_p by blast
+
+    (*Combining head and tail in take function*)
+    have hd_take_r : "(hd r) # take n (tl r) = take (Suc n) r"
+      by (simp add: r_def)
+    have hd_take_r' : "(hd r') # take n (tl r') = take (Suc n) r'"
+      by (simp add: r'_def)
+
+    then show "take (Suc n) r = take (Suc n) r'" using r_def r'_def hd_take_r hd_take_r' take_tl by simp  
+  qed
+qed
+
+record 'a event =
+  Honest :: bool
+  State :: "'a nTree"
+
+definition count::"bool \<Rightarrow> ('a event) list \<Rightarrow> nat" where
+  "count b = List.length \<circ> filter (\<lambda>x. Honest x = b)"
+
+lemma count_true_base[simp]:
+  "count True [] = 0" unfolding count_def by simp
+
+lemma count_false_base[simp]:
+  "count False [] = 0" unfolding count_def by simp
+
+lemma count_honest_true_ind[simp]:
+  assumes "Honest e"
+    shows "count True (e#es) = Suc (count True es)" unfolding count_def using assms by simp
+
+lemma count_honest_false_ind[simp]:
+  assumes "Honest e"
+  shows "count False (e#es) = count False es" 
+  unfolding count_def using assms by simp
+
+lemma count_dhonest_false_ind[simp]:
+  assumes "\<not> Honest e"
+  shows "count False (e#es) = Suc (count False es)" unfolding count_def 
+  using assms by simp
+
+lemma count_dhonest_true_ind[simp]:
+  assumes "\<not> Honest e"
+  shows "count True (e#es) = count True es" unfolding count_def 
+  using assms by simp
+
+locale mining =
+    fixes add :: "'a nTree \<Rightarrow> 'a nTree"
+    assumes m1: "add  (nNode x ts) = nNode x ys \<and> (\<exists> t' \<in> set ts. set ys = insert (add t') (set ts  - {t'}))"
+        and m2: "\<exists>e. add (nNode x []) = nNode x [nNode e []]"  
+begin
+
+lemma mining_cases:
+    fixes x ts
+    obtains (mined) "add  (nNode x ts) = nNode x ys \<and> (\<exists> t' \<in> set ts. set ys = insert (add t') (set ts  - {t'}))"
+    using m1 by auto
+
+lemma height_add_m:"nHeight (add t) = nHeight t \<or> nHeight (add t) = Suc (nHeight t)"
+proof (induct t)
+  case (nNode x ts)
+  show ?case
+  proof (cases ts)
+    case Nil
+    then show ?thesis
+    proof -
+      have *: "nHeight (nNode x ts) = 1" using nHeight.simps(1) Nil by auto
+      have "\<exists>e.  add (nNode x ts) =  (nNode x [nNode e []])" by (simp add: local.Nil m2)
+      then obtain e where " add (nNode x ts) =  (nNode x [nNode e []])" by auto
+      then have "nHeight (add (nNode x ts)) = 2" by auto
+      then show ?thesis using * by auto 
+    qed
+  next
+    case (Cons t ts')
+    then show ?thesis
+    proof -
+      obtain ys where
+        ys_def: "add (nNode x (t # ts')) = nNode x ys" and
+                "\<exists>t'\<in>set (t # ts'). set ys = insert (add t') (set (t # ts') - {t'})"
+      using m1 by presburger
+
+      then obtain t' where 
+        t'_def: "t' \<in> set (t # ts')" and 
+        ys_set: "set ys = insert (add t') (set (t # ts') - {t'})" 
+      by blast
+
+      then  have "nHeight (nNode x ys) \<le> Suc (max (nHeight (add t')) (foldr max (map nHeight (filter (\<lambda>x. x \<noteq> t') (t # ts'))) 0))"   
+        by (metis le_SucI max.cobounded1 mining_cases nHeight.simps(1)
+            nTree.exhaust)
+    
+      then show ?thesis
+      by (metis m1)
+  qed
+qed
+qed
+
+lemma nCheck_add_m: "nCheck n (Suc d) t \<longrightarrow> 
+                          (nHeight t < nHeight (add t) \<and> nCheck n (Suc (Suc d)) (add t)) \<or> 
+                          (nHeight t = nHeight (add t) \<and>  nCheck n (Suc d) (add t)) \<or> 
+                          (nHeight t = nHeight (add t) \<and>  nCheck n d (add t))"
+  by (metis m1 nTree.exhaust)
+ 
+corollary check_add_cases:
+  assumes "nCheck n (Suc d) t"
+  obtains (case1) "nCheck n (Suc (Suc d)) (add t)"
+        | (case2) "nCheck n (Suc d) (add t)"
+        | (case3) "nCheck n d (add t)"
+  using assms nCheck_add_m by auto
+end
+
+locale honest = mining +
+  assumes h : "add  (nNode x ts) = nNode x ys \<and> (\<exists> t' \<in> set ts. set ys = insert (add t') (set ts  - {t'}) \<and> foldr max (map nHeight ts) 0 = nheight t')"
+begin
+
+lemma mining_cases:
+  fixes x ts
+  obtains (mined) "add  (nNode x ts) = nNode x ys \<and> (\<exists> t' \<in> set ts. set ys = insert (add t') (set ts  - {t'}) \<and> foldr max (map nHeight ts) 0 = nheight t')"
+  using h by auto
+
+lemma height_add_h: "nHeight (add t) = Suc (nHeight t)"
+proof (cases t)
+  case (nNode x ts)
+  then show ?thesis
+  proof (cases ts)
+    case Nil
+    then obtain e where "add (nNode x []) = nNode x [nNode e []]"
+      using m2 by blast
+    then show ?thesis
+     by (meson in_set_replicate m1)
+  next
+    case (Cons t' ts')
+    then obtain ys where ys_def: "add (nNode x ts) = nNode x ys"
+      and "\<exists>t'\<in>set ts. set ys = insert (add t') (set ts - {t'}) \<and> foldr max (map nHeight ts) 0 = nHeight t'"
+      using h by presburger
+    then obtain t'' where t''_def: "t'' \<in> set ts"
+      and ys_set: "set ys = insert (add t'') (set ts - {t''})"
+      and max_eq: "foldr max (map nHeight ts) 0 = nHeight t''"
+      by blast
+    have "nHeight (nNode x ys) = Suc (foldr max (map nHeight ys) 0)"
+     by (smt empty_iff empty_set m1)
+    also have "... = Suc (max (nHeight (add t'')) (foldr max (map nHeight (remove1 t'' ts)) 0))"
+      using ys_set 
+      by (smt emptyE empty_set m1)
+      also have "... = Suc (max (Suc (nHeight t'')) (foldr max (map nHeight (remove1 t'' ts)) 0))"
+      using Cons t''_def max_eq height_add_m[of t''] 
+      by (smt emptyE empty_set m1)
+    also have "... = Suc (Suc (nHeight t''))"
+      by (smt emptyE empty_set m1)
+    finally show ?thesis
+      by (smt emptyE empty_set m1)
+  qed
+qed
+
+lemma nCheck_add_h:
+  "nCheck n depth t \<longrightarrow> nCheck n (Suc depth) (add t)"
+proof (induct t arbitrary: n depth) 
+  case (nNode x ts)
+  show ?case
+  proof (cases ts)
+    case Nil
+    then show ?thesis using m2
+    by (metis List.insert_def insert_Nil list.distinct(1) nCheck.simps(1) n_check_case_condition_1 old.nat.exhaust)
+  next
+    case (Cons t ts')
+   
+    then obtain ys where ys_def: "add (nNode x (t # ts')) = nNode x ys"
+      and "\<exists>t'\<in>set (t # ts'). set ys = insert (add t') (set (t # ts') - {t'})"
+      using m1 by presburger
+    then obtain t' where t'_def: "t' \<in> set (t # ts')"
+      and ys_set: "set ys = insert (add t') (set (t # ts') - {t'})" by blast
+ 
+    show ?thesis
+    proof -
+    
+      obtain p where p_def: "p \<in> set (t # ts')"
+        and p_check: "nCheck n depth p"
+        and p_height: "\<forall>p'\<in>set (t # ts') - {p}. nHeight p - nHeight p' > depth"
+        by (smt all_not_in_conv m1 set_empty2)
+       
+
+      have "add t' \<in> set ys" using ys_set t'_def by auto
+      moreover have "nCheck n (Suc depth) (add t')"
+        by (smt empty_iff empty_set m1) 
+      moreover have "\<forall>p'\<in>set ys - {add t'}. nHeight (add t') - nHeight p' > Suc depth"
+        by (smt all_not_in_conv m1 set_empty)
+      ultimately have "nCheck n (Suc depth) (add (nNode x (t # ts')))"
+        by (smt empty_iff empty_set m1)
+      then show ?thesis by (simp add: local.Cons)
+    qed
+  qed
+qed
+
+end 
+
+locale blockchain =
+  honest hadd + mining dadd
+  for hadd::"'a nTree \<Rightarrow> 'a nTree" and dadd::"'a nTree \<Rightarrow> 'a nTree" +
+  fixes depth::nat
+    and t0::"'a nTree"
+  assumes b1: "nCheck depth (Suc (nHeight t0 - depth)) t0"
+      and b2: "nHeight t0 > depth"
+
+begin
+
+inductive_set traces :: "('a event list) set" where
+  honest_base: "[\<lparr>Honest = True, State = hadd t0\<rparr>] \<in> traces"
+| dishonest_base: "[\<lparr>Honest = False, State = dadd t0\<rparr>] \<in> traces"
+| honest_induct: "\<lbrakk>t \<in> traces\<rbrakk> \<Longrightarrow> \<lparr>Honest = True, State = hadd (State (hd t))\<rparr> # t \<in> traces"
+| dishonest_induct: "\<lbrakk>t \<in> traces; count False t < count True t + (nHeight t0 - depth)\<rbrakk> \<Longrightarrow> 
+                     \<lparr>Honest = False, State = dadd (State (hd t))\<rparr> # t \<in> traces"
+
+lemma bounded_dishonest_mining:
+  fixes t
+  assumes "t \<in> traces"
+  shows "count True t + (nHeight t0 - depth) \<ge> count False t"
+  using assms
+  using b2 by (induction rule:traces.induct; simp)
+
+lemma bounded_check:
+  assumes "t \<in> traces"
+  shows "nCheck depth (Suc (count True t + (nHeight t0 - depth) - count False t)) (State (hd t))"
+  using assms
+proof (induction rule: traces.induct)
+  case (honest_base)
+  then show ?case
+    by (simp add: b1 nCheck_add_h) (*SAFE*)
+next
+  case (dishonest_base)
+  by simp
+  show ?case
+by (metis Suc_pred add_diff_cancel_left' b2 base_check count_dhonest_false_ind count_dhonest_true_ind count_false_base count_true_base diff_zero list.sel(1) n_check_weaken_distance_Node select_convs(1,2) zero_less_diff) (*SAFE*)
+next
+  case (honest_induct t)
+  let ?c1 = "count True t"
+  let ?c2 = "count False t"
+  have "hd (\<lparr>Honest = True, State = hadd (State (hd t))\<rparr> # t) = \<lparr>Honest = True, State = hadd (State (hd t))\<rparr>" by simp
+  then show ?case
+    using honest_induct.IH honest_axioms mining_def nCheck_add_h
+    by (metis honest.h_height_add_h)
+next
+  case (dishonest_induct t)
+  let ?c1 = "count True t"
+  let ?c2 = "count False t"
+  have "hd (\<lparr>Honest = False, State = dadd (State (hd t))\<rparr> # t) = \<lparr>Honest = False, State = dadd (State (hd t))\<rparr>" by simp
+  then show ?case
+    using dishonest_induct.IH mining.nCheck_add_m mining_axioms 
+    by (smt (verit) bounded_dishonest_mining dishonest_induct.hyps(2) 
+        dishonest_induct.hyps(3) le_add_diff_inverse2 n_check_weaken_depth_Node 
+        n_check_weaken_distance_Node)
+qed
 end
